modify Balloc's [alloc_gen] and [free_gen] to support both [list2mem] and [list2nmem]
[BALLOC.rep_gen] now has two predicate arguments: one that is useful
for [list2mem] memories, and one that is useful for [list2nmem] memories.

src/Balloc.v
@@ -249,21 +249,25 @@ Module BALLOC.
   Definition alloc_gen := alloc'.
   Definition free_gen := free'.
 
-  Definition rep_gen V xp (freeblocks : list addr) (genpred : @pred _ (@weq addrlen) V) :=
+  Definition rep_gen V xp (freeblocks : list addr)
+                          (genpred : @pred _ (@weq addrlen) V)
+                          (genpredn : @pred _ eq_nat_dec V) :=
     (exists bmap,
      rep' xp bmap *
      [[ forall a, In a freeblocks <-> bmap a = Avail ]] *
-     [[ genpred = listpred (fun a => a |->?) freeblocks ]])%pred.
+     [[ genpred = listpred (fun a => a |->?) freeblocks ]] *
+     [[ genpredn = listpred (fun a => #a |->?) freeblocks ]])%pred.
 
   Theorem alloc_gen_ok : forall V lxp xp mscs,
-    {< Fm mbase m freeblocks genpred,
+    {< Fm mbase m freeblocks genpred genpredn,
     PRE            MEMLOG.rep lxp (ActiveTxn mbase m) mscs *
-                   [[ (Fm * @rep_gen V xp freeblocks genpred)%pred (list2mem m) ]]
+                   [[ (Fm * @rep_gen V xp freeblocks genpred genpredn)%pred (list2mem m) ]]
     POST:(mscs',r) [[ r = None ]] * MEMLOG.rep lxp (ActiveTxn mbase m) mscs' \/
-                   exists bn m' freeblocks' genpred', [[ r = Some bn ]] *
+                   exists bn m' freeblocks' genpred' genpredn', [[ r = Some bn ]] *
                    MEMLOG.rep lxp (ActiveTxn mbase m') mscs' *
-                   [[ (Fm * @rep_gen V xp freeblocks' genpred')%pred (list2mem m') ]] *
+                   [[ (Fm * @rep_gen V xp freeblocks' genpred' genpredn')%pred (list2mem m') ]] *
                    [[ genpred =p=> genpred' * bn |->? ]] *
+                   [[ genpredn =p=> genpredn' * #bn |->? ]] *
                    [[ valid_block xp bn ]]
     CRASH          MEMLOG.log_intact lxp mbase
     >} alloc_gen lxp xp mscs.
@@ -282,7 +286,7 @@ Module BALLOC.
     pred_apply.
     cancel.
 
-    assert (a a3 = Avail) as Ha by ( apply H8; eapply remove_still_In; eauto ).
+    assert (a a3 = Avail) as Ha by ( apply H9; eapply remove_still_In; eauto ).
     rewrite <- Ha.
     apply fupd_other.
     eapply remove_still_In_ne; eauto.
@@ -291,21 +295,26 @@ Module BALLOC.
     intro He. subst. rewrite fupd_same in *. discriminate. trivial.
     rewrite fupd_other in * by assumption.
     apply remove_other_In. assumption.
-    rewrite H8; assumption.
+    rewrite H9; assumption.
 
     erewrite listpred_remove with (dec := @weq addrlen). cancel.
-    apply ptsto_conflict.
-    rewrite H8; assumption.
+    intros; apply ptsto_conflict.
+    rewrite H9; assumption.
+
+    erewrite listpred_remove with (dec := @weq addrlen). cancel.
+    intros; apply ptsto_conflict.
+    rewrite H9; assumption.
   Qed.
 
   Theorem free_gen_ok : forall V lxp xp bn mscs,
-    {< Fm mbase m freeblocks genpred,
+    {< Fm mbase m freeblocks genpred genpredn,
     PRE        MEMLOG.rep lxp (ActiveTxn mbase m) mscs *
-               [[ (Fm * @rep_gen V xp freeblocks genpred)%pred (list2mem m) ]] *
+               [[ (Fm * @rep_gen V xp freeblocks genpred genpredn)%pred (list2mem m) ]] *
                [[ (bn < BmapNBlocks xp ^* $ valulen)%word ]]
-    POST:mscs' exists m' genpred', MEMLOG.rep lxp (ActiveTxn mbase m') mscs' *
-               [[ (Fm * @rep_gen V xp (bn :: freeblocks) genpred')%pred (list2mem m') ]] *
-               [[ bn |->? * genpred =p=> genpred' ]]
+    POST:mscs' exists m' genpred' genpredn', MEMLOG.rep lxp (ActiveTxn mbase m') mscs' *
+               [[ (Fm * @rep_gen V xp (bn :: freeblocks) genpred' genpredn')%pred (list2mem m') ]] *
+               [[ bn |->? * genpred =p=> genpred' ]] *
+               [[ #bn |->? * genpredn =p=> genpredn' ]]
     CRASH      MEMLOG.log_intact lxp mbase
     >} free_gen lxp xp bn mscs.
   Proof.
@@ -316,25 +325,25 @@ Module BALLOC.
     cancel.
     step.
     subst; apply fupd_same; trivial.
-    rewrite H9 in H3.
+    rewrite H10 in H3.
     destruct (weq bn a1).
     subst; apply fupd_same; trivial.
     rewrite <- H3; apply fupd_other; assumption.
     destruct (weq bn a1).
     left. auto.
-    right. rewrite fupd_other in H0 by assumption. apply H9; assumption.
+    right. rewrite fupd_other in H0 by assumption. apply H10; assumption.
   Qed.
 
   Hint Extern 1 ({{_}} progseq (BALLOC.alloc_gen _ _ _) _) => apply BALLOC.alloc_gen_ok : prog.
   Hint Extern 1 ({{_}} progseq (BALLOC.free_gen _ _ _ _) _) => apply BALLOC.free_gen_ok : prog.
-  Hint Extern 0 (okToUnify (rep_gen _ _ _) (rep_gen _ _ _)) => constructor : okToUnify.
+  Hint Extern 0 (okToUnify (rep_gen _ _ _ _) (rep_gen _ _ _ _)) => constructor : okToUnify.
 
   (* Different names for actual on-disk-block allocation *)
   Definition alloc := alloc_gen.
   Definition free := free_gen.
 
   Definition rep xp (freeblocks : list addr) :=
-    (exists genpred, genpred * rep_gen xp freeblocks genpred)%pred.
+    (exists genpred genpredn, genpred * rep_gen xp freeblocks genpred genpredn)%pred.
 
   Theorem alloc_ok : forall lxp xp mscs,
     {< Fm mbase m freeblocks,
@@ -352,7 +361,7 @@ Module BALLOC.
     eapply pimpl_ok2. apply alloc_gen_ok.
     cancel.
     step.
-    rewrite H9 in H0.
+    rewrite H10 in H7.
     apply pimpl_or_r. right.
     cancel.
   Qed.
